Splinter/AllocationsLayer/CoordinationSystemRefinement.i.dfy
@@ -1,0 +1,140 @@
+// Copyright 2018-2021 VMware, Inc., Microsoft Inc., Carnegie Mellon University, ETH Zurich, and University of Washington
+// SPDX-License-Identifier: BSD-2-Clause
+
+include "CoordinationSystem.i.dfy"
+include "FullStackBetreeRefinement.i.dfy"
+include "FullStackJournalRefinement.i.dfy"
+
+module CoordinationSystemRefinement {
+  import opened GenericDisk
+  import FullStackJournalRefinement
+  import FullStackBetreeRefinement
+  import opened CoordinationSystemMod
+  import AllocationBetreeMod
+  // import AbstractSystem = CoordinationSystem
+//   import opened Options
+//   import opened MapRemove_s
+//   import opened CrashTolerantMapSpecMod
+//   import opened MsgHistoryMod
+//   import opened KeyType
+//   import opened ValueMessage
+//   import opened TotalKMMapMod
+//   import opened LSNMod
+//   import opened CoordinationJournal
+//   import opened CoordinationBetree
+
+  predicate KnownEphemeral(v: Variables)
+  {
+    && v.journal.ephemeral.Known? 
+    && v.betree.ephemeral.Known?
+  }
+
+  predicate InFlightReady(v: Variables)
+  {
+    && v.journal.inFlight.Some? 
+    && v.betree.inFlight.Some? 
+    && v.freeset.inFlight.Some? 
+  }
+
+  predicate DisjointEphemeralComponents(v: Variables)
+  {
+    && (KnownEphemeral(v) ==> v.freeset.ephemeral !! v.betree.EphemeralAUs() !! v.journal.EphemeralAUs())
+  }
+
+  // betree journal freeze differently
+  predicate DisjointInFlightComponents(v: Variables)
+  {
+    // NOTE: journal's inflight AU just into existence at a later time, might make this hard to prove
+    // frozen journal is a subset of the ephemeral journal
+    // ephemeral journal AU !! v.freeset.ephemeral
+    // v.freeset.inflight.value = old v.freeset.ephemeral + frozen freeset data 
+    && (InFlightReady(v) ==> v.freeset.inFlight.value !! v.betree.InFlightAUs() !! v.journal.InFlightAUs())
+  }
+
+  predicate DisjointPersistentComponents(v: Variables)
+  {
+    && v.freeset.persistent !! v.betree.PersistentAUs() !! v.journal.PersistentAUs()
+  }
+
+  function TotalEphemeral(v: Variables) : set<AU>
+    requires KnownEphemeral(v)
+  {
+    v.freeset.ephemeral + v.betree.EphemeralAUs() + v.journal.EphemeralAUs()
+  }
+
+  function TotalPersistent(v: Variables) : set<AU>
+  {
+    v.freeset.persistent + v.betree.PersistentAUs() + v.journal.PersistentAUs()
+  }
+
+  function TotalInflight(v: Variables) : set<AU>
+    requires InFlightReady(v)
+  {
+    v.freeset.inFlight.value + v.betree.InFlightAUs() + v.journal.InFlightAUs()
+  }
+
+  predicate StatesPreservesTotalAUs(v: Variables)
+  {
+    && (KnownEphemeral(v) ==> TotalEphemeral(v) == TotalPersistent(v))
+    && (InFlightReady(v) ==> TotalInflight(v) == TotalPersistent(v))
+  }
+
+  predicate Inv(v: Variables)
+  {
+    && (v.journal.ephemeral.Known? <==> v.betree.ephemeral.Known?)
+    && (v.freeset.inFlight.Some? <==> v.betree.inFlight.Some? && v.journal.inFlight.Some?)
+
+    && FullStackJournalRefinement.Inv(v.journal)
+    && FullStackBetreeRefinement.Inv(v.betree)
+
+    && DisjointEphemeralComponents(v)
+    && DisjointInFlightComponents(v)
+    && DisjointPersistentComponents(v)
+    && StatesPreservesTotalAUs(v)
+  }
+
+  function I(v: Variables) : AbstractSystem.Variables
+    requires Inv(v)
+  {
+    var journal := FullStackJournalRefinement.I(v.journal);
+    var mapadt := FullStackBetreeRefinement.I(v.betree);
+    AbstractSystem.Variables(journal, mapadt, v.ephemeral)
+  } 
+
+  lemma InitRefines(v: Variables, availAUs: set<AU>)
+    requires Init(v, availAUs)
+    ensures Inv(v)
+    ensures AbstractSystem.Init(I(v))
+  {
+    FullStackBetreeRefinement.InitRefines(v.betree);
+  }
+
+  lemma NextRefines(v: Variables, v': Variables, uiop: UIOp)
+    requires Inv(v)
+    requires Next(v, v', uiop)
+    ensures Inv(v')
+    ensures AbstractSystem.Next(I(v), I(v'), uiop)
+  {
+    var step :| NextStep(v, v', uiop, step);
+    match step {
+      // case LoadEphemeralFromPersistentStep() => LoadEphemeralFromPersistent(v, v', uiop)
+      // case RecoverStep(records) => Recover(v, v', uiop, records)
+      // case AcceptRequestStep() => AcceptRequest(v, v', uiop)
+      // case QueryStep() => Query(v, v', uiop)
+      // case PutStep() => Put(v, v', uiop)
+      // case DeliverReplyStep() => DeliverReply(v, v', uiop)
+      // case JournalInternalStep(allocs, deallocs) => JournalInternal(v, v', uiop, allocs, deallocs)
+      // case MapInternalStep(allocs, deallocs) => MapInternal(v, v', uiop, allocs, deallocs)
+      // case ReqSyncStep() => ReqSync(v, v', uiop)
+      // case ReplySyncStep() => ReplySync(v, v', uiop)
+      // case FreezeBetreeStep(unobservedBetree, unobservedJournal) => FreezeBetree(v, v', uiop, unobservedBetree, unobservedJournal)
+      // case CommitStartStep(newBoundaryLsn) => CommitStart(v, v', uiop, newBoundaryLsn)
+      // case CommitCompleteStep(discardedJournal) => CommitComplete(v, v', uiop, discardedJournal)
+      // case CrashStep() => Crash(v, v', uiop)
+      case _ => assume false;
+    }
+    // requires lbl.InternalLabel? ==> AllocationBetreeRefinement.FreshLabel(v.ephemeral.v, AllocLbl(v, v', lbl))
+    // FullStackBetreeRefinement.NextRefines(v.betree, v'.betree);
+    // FullStackJournalRefinement.NextRefines(v.journal, v'.journal);
+  }
+}
